verificacion con is_heap de operaciones. wip number_nodes0

BinomialHeap.fst
@@ -7,35 +7,10 @@ open InsertionSort
 
 type node0 = | N of nat & int & list node0 // rank, data, children
 
-let rank (tree : node0) : nat =
-  let N (r,_,_) = tree in
-  r
-
-let root (tree : node0) : int =
-  let N (_,r,_) = tree in
-  r
-
-let children (tree : node0) : list node0 =
-  let N (_,_,c) = tree in
-  c
-
-let singleton (x: int): node0 = N (0, x, [])
-
-let link (tree1 tree2 : node0) : node0 =
-  match tree1, tree2 with
-  | N (r, k1, c1), N (_, k2, c2) -> if k1 <= k2
-                                    then N (r + 1, k1, tree2 :: c1)
-                                    else N (r + 1, k2, tree1 :: c2)
-
-let rec all_nodes (#a:Type) (#b: Type) (bound : a) (f: (x:node0{x << bound}) -> b) (op: b -> b -> b) (e: b) (l: list node0{l << bound}) : b = 
-  match l with
-    | [] -> e
-    | x::xs -> op (f x) (all_nodes bound f op e xs)
-
-let rec all_le0 (x: int) (tree: node0) : bool =
+let rec all_le0 (x: int) (tree: node0) : Tot bool (decreases %[tree; 0])=
   match tree with
-  | N (r, k, c) -> k <= x && all_le x c
-and all_le (x: int) (bh: list node0) : bool =
+  | N (r, k, c) -> x <= k && all_le k c
+and all_le (x: int) (bh: list node0) : Tot bool (decreases %[bh; 1])=
   match bh with
     | [] -> true
     | h::hs -> all_le0 x h && all_le x hs
@@ -48,11 +23,66 @@ and is_heap (bh: list node0) : bool =
     | [] -> true
     | h::hs -> is_heap0 h && is_heap hs
 
+let rank0 (tree : node0) : nat =
+  let N (r,_,_) = tree in
+  r
+
+let root0 (tree : node0) : int =
+  let N (_,r,_) = tree in
+  r
+
+let children0 (tree : node0) : list node0 =
+  let N (_,_,c) = tree in
+  c
+
+type node = n:node0{is_heap0 n}
+
+let singleton (x: int): node = N (0, x, [])
+
+let link0 (tree1 : node0) (tree2 : node0{rank0 tree1 = rank0 tree2}) : node0 =
+  match tree1, tree2 with
+  | N (r, k1, c1), N (_, k2, c2) -> if k1 <= k2
+                                    then N (r + 1, k1, tree2 :: c1)
+                                    else N (r + 1, k2, tree1 :: c2)
+
+let link0_all_le (x: int) (tree1 : node0) (tree2 : node0{rank0 tree1 = rank0 tree2}) :
+  Lemma (requires all_le0 x tree1 /\ all_le0 x tree2)
+        (ensures all_le0 x (link0 tree1 tree2))
+= ()
+
+let append_is_heap (tree1 : node0) (tree2 : node0{rank0 tree1 = rank0 tree2}) : 
+  Lemma (requires is_heap0 tree1 /\ is_heap0 tree2)
+        (ensures is_heap (tree2::(children0 tree1)))
+= ()
+  
+let is_heap0_all_le0 (tree1 tree2: node0) : 
+  Lemma (requires is_heap0 tree1 /\ is_heap0 tree2 /\ root0 tree1 <= root0 tree2)
+        (ensures all_le0 (root0 tree1) tree2)
+= ()
+let link0_is_heap0 (tree1 : node0) (tree2 : node0{rank0 tree1 = rank0 tree2}) : 
+  Lemma (requires is_heap0 tree1 /\ is_heap0 tree2)
+        (ensures is_heap0 (link0 tree1 tree2))
+= match tree1, tree2 with
+  | N (r, k1, c1), N (_, k2, c2) -> if k1 <= k2
+                                    then (
+                                      assert(is_heap (tree2::c1));
+                                      assert(all_le0 k1 tree2)
+                                    )
+                                    else (
+                                      assert(is_heap (tree1::c2));
+                                      assert(all_le0 k2 tree1)
+                                    )
+
+let link (tree1 : node) (tree2 : node{rank0 tree1 = rank0 tree2}) : node 
+=
+  link0_is_heap0 tree1 tree2;
+  link0 tree1 tree2
+
 let rec incr_rank (hs : list node0) : prop =
   match hs with
   | [] -> True
   | [_] -> True
-  | h1::h2::hs' -> rank h1 < rank h2 /\ incr_rank (h2::hs')
+  | h1::h2::hs' -> rank0 h1 < rank0 h2 /\ incr_rank (h2::hs')
 
 let rec number_nodes0 (tree: node0) : nat =
   match tree with
@@ -62,7 +92,7 @@ and number_nodes (bh: list node0) : nat =
     | [] -> 0
     | h::hs -> number_nodes0 h + number_nodes hs
 
-type bheap = list node0
+type bheap = list node
 
 let emptyHeap : bheap = []
 
@@ -71,12 +101,12 @@ let isEmptyHeap (h: bheap) : bool =
   | [] -> true
   | _ -> false
 
-let rec insertTree (t: node0) (bh: bheap) : Tot bheap (decreases (length bh))=
+let rec insertTree (t: node) (bh: bheap) : Tot bheap (decreases (length bh))=
   match bh with
   | [] -> [t]
-  | h::hs -> if rank t < rank h
+  | h::hs -> if rank0 t < rank0 h
              then t::bh
-             else if rank t = rank h
+             else if rank0 t = rank0 h
                   then insertTree (link t h) hs
                   else h :: insertTree t hs
 
@@ -87,23 +117,23 @@ let rec merge (bh1: bheap) (bh2: bheap) : bheap =
   match bh1, bh2 with
   | [], _ -> bh2
   | _, [] -> bh1
-  | h1::hs1, h2::hs2 -> if rank h1 < rank h2
+  | h1::hs1, h2::hs2 -> if rank0 h1 < rank0 h2
                         then h1 :: merge hs1 bh2
-                        else if rank h1 > rank h2
+                        else if rank0 h1 > rank0 h2
                              then h2 :: merge bh1 hs2
                              else insertTree (link h1 h2) (merge hs1 hs2)
 
-let rec removeMinTree (bh: bheap{Cons? bh}) : (node0 & bheap)  =
+let rec removeMinTree (bh: bheap{Cons? bh}) : (node & bheap)  =
   match bh with
   | [h] -> (h, [])
   | h::hs -> let m, hs' = removeMinTree hs in
-             if root h < root m
+             if root0 h < root0 m
              then (h, hs)
              else (m, h::hs')
 
 
 let findMin (bh: bheap{Cons? bh}) : int =
-  let m, _ = removeMinTree bh in root m
+  let m, _ = removeMinTree bh in root0 m
 
 let rec rev_go #a (acc xs : list a) : Tot (list a) (decreases xs)=
   match xs with
@@ -113,9 +143,15 @@ let rec rev_go #a (acc xs : list a) : Tot (list a) (decreases xs)=
 let rev (#a:Type) (xs : list a) : list a =
   rev_go [] xs
 
+let rec children (n: node) : Tot (list node) (decreases (number_nodes0 n))
+= 
+  match n with
+    | N (_,_,[]) -> []
+    | N (r,k, c::cs) -> c :: children (N (r, k, cs))
+
 let extractMin (bh: bheap{Cons? bh}) : int & bheap =
-  let m, hs = removeMinTree bh in
-  root m, merge (rev (children m)) hs
+  let m, hs = removeMinTree bh in 
+  root0 m, merge (rev (children m)) hs
 
 let rec lemma_removeMinTree_size (bh : bheap{Cons? bh})
   : Lemma (number_nodes bh == number_nodes (snd (removeMinTree bh)) + number_nodes0 (fst (removeMinTree bh)))
@@ -142,9 +178,9 @@ let rec lemma_insertTree_size (tree: node0) (bh: bheap)
   = 
     match bh with
     | [] -> ()
-    | h::hs -> if rank tree < rank h
+    | h::hs -> if rank0 tree < rank0 h
                then ()
-               else if rank tree = rank h
+               else if rank0 tree = rank0 h
                     then lemma_insertTree_size (link tree h) hs
                     else lemma_insertTree_size tree hs
 
@@ -154,9 +190,9 @@ let rec lemma_merge_size (bh1 bh2: bheap)
     match bh1, bh2 with
     | [], _ -> ()
     | _, [] -> ()
-    | h1::hs1, h2::hs2 -> if rank h1 < rank h2
+    | h1::hs1, h2::hs2 -> if rank0 h1 < rank0 h2
                           then lemma_merge_size hs1 bh2
-                          else if rank h1 > rank h2
+                          else if rank0 h1 > rank0 h2
                                then lemma_merge_size bh1 hs2
                                else (
                                      lemma_insertTree_size (link h1 h2) (merge hs1 hs2); 
@@ -186,6 +222,19 @@ let rec toList (bh: bheap) : Tot (list int) (decreases (number_nodes bh))=
            lemma_deleteMin_size bh;
            m :: toList bh'
 
+let rec elems_node0 (n: node0) : list int =
+  let N (x, _, c) = n in
+  x :: elems_nodes c
+and elems_nodes (cs: list node0) : list int =
+  match cs with
+    | [] -> []
+    | c::cs' -> elems_node0 c @ elems_nodes cs'
+
+let rec toList2 (bh: bheap) : Tot (list int) (decreases (number_nodes bh))=
+  match bh with
+    | [] -> []
+    | h::hs -> elems_node0 h @ toList2 hs 
+
 let rec fromList (l: list int) : bheap =
   match l with
     | [] -> []
@@ -194,9 +243,8 @@ let rec fromList (l: list int) : bheap =
 let models (bh : bheap) (xs : list int) : prop =
   toList bh == xs
 
-val insert_ok  (bh : bheap) (x : int) (xs : list int)
-  : Lemma (requires models bh xs)
-          (ensures models (insert x bh) (insertion_sort (<) (x :: xs)))
+let models2 (bh : bheap) (xs : list int) : prop =
+  perm (toList2 bh) xs
 
 val findMin_ok (bh : bheap) (x : int) (xs : list int)
   : Lemma (requires models bh (x::xs))
@@ -207,9 +255,29 @@ val deleteMin_ok (bh : bheap) (x : int) (xs : list int)
           (ensures models (snd (extractMin bh)) xs)
 
 let findMin_ok (bh : bheap) (x : int) (xs : list int)
-  : Lemma (requires models bh (x::xs))
-          (ensures findMin bh == x) = ()
+  : Lemma (requires models bh xs)
+          (ensures findMin bh == findMin_list xs) = ()
 
 let deleteMin_ok (bh : bheap) (x : int) (xs : list int)
   : Lemma (requires models bh (x::xs))
           (ensures models (snd (extractMin bh)) xs) = ()
+
+val insert_ok  (bh : bheap) (x : int) (xs : list int)
+  : Lemma (requires models bh xs)
+          (ensures models (insert x bh) (InsertionSort.insert (<=) x xs))
+
+assume val merge_sort (xs ys: list int) : list int
+
+assume val merge_ok (bh1 bh2: bheap) (xs ys: list int) 
+  : Lemma (requires models bh1 xs /\ models bh2 ys)
+          (ensures models (merge bh1 bh2) (merge_sort xs ys))
+
+let insert_ok  (bh : bheap) (x : int) (xs : list int)
+  : Lemma (requires models bh xs)
+          (ensures models (insert x bh) (insertion_sort (<=) (x :: xs)))
+= assert([singleton x] `models` [x]); 
+  merge_ok [singleton x] bh [x] xs; 
+  assert (merge [singleton x] bh `models` (merge_sort [x] xs));
+  assert (insert x bh `models` (merge_sort [x] xs));
+  assert (insert x bh `models` (InsertionSort.insert (<=) x xs));
+  admit()
